hfc/MMHighStageOne.v
@@ -52,7 +52,10 @@ Require Import Types.
 Require Import MpoolConcur.
 Require Import ArchMM.
 Require Import Lock.
-        
+
+(* This is to define abstract types *)
+Require Import IntMap.Map.
+
 
 Import LangNotations.
 
@@ -91,349 +94,32 @@ Notation "x <- c1 ;; c2" := (@pbind _ (PMonad_Monad Monad_option) _ _ _ c1 (fun 
                               (at level 61, c1 at next level, right associativity).
 Require Import Any.
 
-Section AbsData.
-
-  (* common definition *)
-
-  Definition ident := N.
-
-  Instance RelDec_ident: RelDec (@eq ident) :=
-    { rel_dec := fun n0 n1 => if (N.eqb n0 n1) then true else false}.
-
-  (* mpool *)
-
-  Record mpool: Type :=
-    mk {
-        chunklist: list (nat * nat); (* paddr, limit *)
-        fallback: option ident; (* mpoolid *)
-      }
-  .
-
-  Definition mp_manager: Type := ident -> option mpool.
-  Definition inital_mp_manager: mp_manager := fun _ => None.
-  Definition mp_update (m: mp_manager) (k0: ident) (v: option mpool): mp_manager :=
-    fun k1 => if rel_dec k0 k1 then v else m k1
-  .
-
-  (* The following are arch-independent page mapping modes. *)
-  Inductive ModeFlag :=
-  | MM_UNDEF1 (* nothing *)
-  | MM_MODE_R (* read *)
-  | MM_MODE_W (* write *)
-  | MM_MODE_X (* execute *)
-  | MM_MODE_D (* device *)
-  .
-
-  
-  Inductive OwnModeFlag :=
-  | MM_UNDEF2
-  | MM_MODE_INVALID
-  | MM_MODE_UNOWNED
-  | MM_MODE_SHARED.
-  
-  
-  (* I do not know whether this one is necessary or not 
-  Inductive AccessFlag :=
-  | AF_USED
-  | AF_NON.
-  *)
-
-  (* This is the wrapper definition for va_addr to distinguish it with normal natural numbers *)
-  Inductive va_addr :=
-  | VA_ADDR (va: N).
-
-  Inductive ipa_addr :=
-  | IPA_ADDR (ipa: N).
-
-  (* Low level functional model for mm_index *)
-  (*
-  Definition mm_index (addr level: var) (v  : var) : stmt :=
-    v #= addr #>> (PAGE_BITS + (level * PAGE_LEVEL_BITS)) #;
-      Return (v #& ((UINT64_C(1) #<< PAGE_LEVEL_BITS) - 1)).
-   *)
-  
-  (* high-level functional model for mm_index - It is quite same. we just change the definition as a normal Coq definition  *)
-  Definition h_mm_index  (va : va_addr) (level : N) : N :=
-    match va with
-    | VA_ADDR va' =>
-      let v := (N.shiftr va' ((level * PAGE_LEVEL_BITS)%N + PAGE_BITS)%N) in
-      let mask := (N.shiftl 1 PAGE_LEVEL_BITS) - 1 in
-      (N.land v mask) 
-    end.
-
-  Definition va_page_bits (va: va_addr) : N :=
-    match va with
-    | VA_ADDR va' =>
-      let mask := (N.shiftl 1 PAGE_BITS) - 1 in
-      (N.land va' mask)
-    end.
-
-  Definition ipa_block_idx (level : N) (ipa : ipa_addr) : N :=
-    match ipa with
-    | IPA_ADDR ipa' =>
-      let mask := (N.shiftl 1 PAGE_LEVEL_BITS) - 1 in
-      (N.land (N.shiftr ipa' ((level * PAGE_LEVEL_BITS)%N + PAGE_BITS)%N) mask) 
-    end.
-
-  
-
-  
-
-  
-  (*
-  MM_FLAG_STAGE1
-    MM_FLAG_COMMIT
-    MM_FLAG_UNMAP
-    MM_MODE_UNMAPPED_MASK
-   *)
-  
-  Inductive ValidFlag :=
-  | MM_VALID
-  | MM_ABSENT.
-
-  Inductive OwnedFlag :=
-  | OWNED
-  | UNOWEND.
-
-  Inductive SharedFlag :=
-  | EXCLUSIVE
-  | SHARED.
-  
-  Inductive SG1Flag :=
-  | SG1_STATUS (val: ValidFlag).
-
-  Inductive SG2Flag :=
-  | SG2_STATUS (val: ValidFlag) (owned: OwnedFlag) (sh: SharedFlag).
 
 
-(*  in ptable_init
-  tables = mm_alloc_page_tables(root_table_count, ppool);
-  if (tables == NULL) {
-    return false;
-  }
 
-  for (i = 0; i < root_table_count; i++) {
-    for (j = 0; j < MM_PTE_PER_PAGE; j++) {
-      tables[i].entries[j] =
-        arch_mm_absent_pte(mm_max_level(flags));
-    }
-  }
- *)
-  
-(*
-uint64_t arch_mm_mode_to_stage2_attrs(uint32_t mode)
-{
-  uint64_t attrs = 0;
-  uint64_t access = 0;
-
-  /*
-   * Non-shareable is the "neutral" share mode, i.e., the shareability
-   * attribute of stage 1 will determine the actual attribute.
-   */
-  attrs |= STAGE2_AF | STAGE2_SH(NON_SHAREABLE);
-
-  /* Define the read/write bits. */
-  if (mode & MM_MODE_R) {
-    access |= STAGE2_ACCESS_READ;
-  }
-
-  if (mode & MM_MODE_W) {
-    access |= STAGE2_ACCESS_WRITE;
-  }
-
-  attrs |= STAGE2_S2AP(access);
-
-  /* Define the execute bits. */
-  if (mode & MM_MODE_X) {
-    attrs |= STAGE2_XN(STAGE2_EXECUTE_ALL);
-  } else {
-    attrs |= STAGE2_XN(STAGE2_EXECUTE_NONE);
-  }
-
-  /*
-   * Define the memory attribute bits, using the "neutral" values which
-   * give the stage-1 attributes full control of the attributes.
-   */
-  if (mode & MM_MODE_D) {
-    attrs |= STAGE2_MEMATTR(STAGE2_DEVICE_MEMORY,
-          STAGE2_MEMATTR_DEVICE_GRE);
-  } else {
-    attrs |= STAGE2_MEMATTR(STAGE2_WRITEBACK, STAGE2_WRITEBACK);
-  }
-
-  /* Define the ownership bit. */
-  if (!(mode & MM_MODE_UNOWNED)) {
-    attrs |= STAGE2_SW_OWNED;
-  }
-
-  /* Define the exclusivity bit. */
-  if (!(mode & MM_MODE_SHARED)) {
-    attrs |= STAGE2_SW_EXCLUSIVE;
-  }
-
-  /* Define the valid bit. */
-  if (!(mode & MM_MODE_INVALID)) {
-    attrs |= PTE_VALID;
-  }
-
-  return attrs;
-}
-*)
- 
- 
-(*  in mm_populate_table_pte
-  /* Allocate a new table. */
-  ntable = mm_alloc_page_tables(1, ppool);
-  if (ntable == NULL) {
-    dlog_error("Failed to allocate memory for page table\n");
-    return NULL;
-  }
-
-  /* Determine template for new pte and its increment. */
-  if (arch_mm_pte_is_block(v, level)) {
-    inc = mm_entry_size(level_below);
-    new_pte = arch_mm_block_pte(level_below,
-              arch_mm_block_from_pte(v, level),
-              arch_mm_pte_attrs(v, level));
-  } else {
-    inc = 0;
-    new_pte = arch_mm_absent_pte(level_below);
-  }
-
-  /* Initialise entries in the new table. */
-  for (i = 0; i < MM_PTE_PER_PAGE; i++) {
-    ntable->entries[i] = new_pte;
-    new_pte += inc;
-  }
- *)
-
- (*
-
-uint32_t arch_mm_stage2_attrs_to_mode(uint64_t attrs)
-{
-  uint32_t mode = 0;
-
-  if (attrs & STAGE2_S2AP(STAGE2_ACCESS_READ)) {
-    mode |= MM_MODE_R;
-  }
-
-  if (attrs & STAGE2_S2AP(STAGE2_ACCESS_WRITE)) {
-    mode |= MM_MODE_W;
-  }
-
-  if ((attrs & STAGE2_XN(STAGE2_EXECUTE_MASK)) ==
-      STAGE2_XN(STAGE2_EXECUTE_ALL)) {
-    mode |= MM_MODE_X;
-  }
-
-  if ((attrs & STAGE2_MEMATTR_TYPE_MASK) == STAGE2_DEVICE_MEMORY) {
-    mode |= MM_MODE_D;
-  }
-
-  if (!(attrs & STAGE2_SW_OWNED)) {
-    mode |= MM_MODE_UNOWNED;
-  }
-
-  if (!(attrs & STAGE2_SW_EXCLUSIVE)) {
-    mode |= MM_MODE_SHARED;
-  }
-
-  if (!(attrs & PTE_VALID)) {
-    mode |= MM_MODE_INVALID;
-  }
-
-  return mode;
-}
-*)
-
-
-(*
-uint64_t arch_mm_mode_to_stage1_attrs(uint32_t mode)
-{
-  uint64_t attrs = 0;
-
-  attrs |= STAGE1_AF | STAGE1_SH(OUTER_SHAREABLE);
-
-  /* Define the execute bits. */
-  if (!(mode & MM_MODE_X)) {
-    attrs |= STAGE1_XN;
-  }
-
-  /* Define the read/write bits. */
-  if (mode & MM_MODE_W) {
-    attrs |= STAGE1_AP(STAGE1_READWRITE);
-  } else {
-    attrs |= STAGE1_AP(STAGE1_READONLY);
-  }
-
-  /* Define the memory attribute bits. */
-  if (mode & MM_MODE_D) {
-    attrs |= STAGE1_ATTRINDX(STAGE1_DEVICEINDX);
-  } else {
-    attrs |= STAGE1_ATTRINDX(STAGE1_NORMALINDX);
-  }
-
-  /* Define the valid bit. */
-  if (!(mode & MM_MODE_INVALID)) {
-    attrs |= PTE_VALID;
-  }
-
-  return attrs;
-}
-*)
-
-
-(*
-uint64_t arch_mm_combine_table_entry_attrs(uint64_t table_attrs,
-             uint64_t block_attrs)
-{
-  /*
-   * Only stage 1 table descriptors have attributes, but the bits are res0
-   * for stage 2 table descriptors so this code is safe for both.
-   */
-  if (table_attrs & TABLE_NSTABLE) {
-    block_attrs |= STAGE1_NS;
-  }
-  if (table_attrs & TABLE_APTABLE1) {
-    block_attrs |= STAGE1_AP2;
-  }
-  if (table_attrs & TABLE_APTABLE0) {
-    block_attrs &= ~STAGE1_AP1;
-  }
-  if (table_attrs & TABLE_XNTABLE) {
-    block_attrs |= STAGE1_XN;
-  }
-  if (table_attrs & TABLE_PXNTABLE) {
-    block_attrs |= STAGE1_PXN;
-  }
-  return block_attrs;
-}
-*)
-
- 
-  
-  (* Do we need them? - those two things - I will skip them at this moment
-  Polymorphic Inductive upper_attrs := | up_attr (val: Type).
-  Polymorphic Inductive low_attrs := | lo_attr (val : Type). *)
-
-  
+Module DummyAbsData.
   
   Inductive PTE_TY :=
   | PTENONE
   | PTE (owner: option N) (paddr : N) (level : N) (vaddr: option N).
+  Instance PTE_TY_Showable: Showable PTE_TY := { show := fun x => match x with
+                                                                  | PTENONE => "PTENONE" |
+                                                                  PTE owner paddr level vaddr => "PTE" 
+                                                                  end }.
 
   Record pt_entry: Type := mkPTE {value: list PTE_TY}.
 
-  Definition pt_manager : Type := ident -> option pt_entry.
-  Definition inital_pt_manager: mp_manager := fun _ => None.
-  Definition pt_update (m: pt_manager) (k0: ident) (v: option pt_entry): pt_manager :=
+  Definition pt_manager : Type := N-> option pt_entry.
+  Definition inital_pt_manager: pt_manager := fun _ => None.
+  Definition pt_update (m: pt_manager) (k0: N) (v: option pt_entry): pt_manager :=
     fun k1 => if rel_dec k0 k1 then v else m k1
   .
 
-End AbsData.
-
+End DummyAbsData.
 
 Module HighSpecDummyTest.
+
+  Include DummyAbsData.
   
   Fixpoint pte_init_iter (base_addr: N) (level : N) (esize : N) (length : nat): list PTE_TY :=
     match length with
@@ -456,52 +142,8 @@ Module HighSpecDummyTest.
                 end
     in (retv, nil).
 
-  (*
-  Definition pte_init_aux2 (vs : list val@{expr.u1}): (val@{expr.u2} * list val@{expr.u3}) :=
-    let retv := match vs with
-                | [(Vabs a)] =>
-                  unwrap (ptes <- downcast a pt_entry ;;
-                          let new_ptes := 
-                              (match ptes with
-                               | mkPTE ptes_v =>
-                                 match dec with
-                                 | O => ptes_v (* use as it is *)
-                                 | _ => pte_init ptes_v 
-                                 end
-                               end) in
-                          Some (Vabs (upcast new_ptes))
-                         ) Vnodef
-                | _ => Vnodef
-                end
-    in (retv, nil).
-    *)
-  
-
-
-  (* JIEUNG: strategy: 
-     MPOOL and PAGE TABLE might have different structures (Is it true?)
-     This prevents us to provide the same abstarct representation. 
-     So, we can duplicate them. 
-     we can initialize two data structures 
-     1. MPOOL 
-     2. PTE  
-     Each one has valid field, which is a logical flag. When we use some parts of memory for page tables, 
-     we will mark that part in MPOOL and PTE together.
-     If it is marked, we can check PTE to see the proper value for page tables. 
-     Diabling them is quite simliar 
-   *)
-  
-  (* JIEUNG: let's make a debugging message for abs types *)
-  (* JIEUNG: let's test the way to build heap *)
-  (*
-  Definition pte_init (d : var) res r : stmt := 
-    r #= GetOwnedHeap #;
-      res #= (CoqCode [CBV r ; CBV d] pte_init_aux) #;
-      PutOwnedHeap r.
-   *)
-
   Definition main res : stmt :=
-    (Debug "[high-model] Calling" Vnull) #;
+    (DebugHigh "[high-model] Calling" Vnull) #;
     res #= (CoqCode [CBV (Vnat 4000) ; CBV (Vnat 1) ; CBV (Vnat 4) ; CBV (Vnat 4)] pte_init) #;
     DebugHigh "[high-model] Calling" res #;
     DebugHigh "[high-model] Call End" res.
@@ -517,125 +159,281 @@ Module HighSpecDummyTest.
     ].
   
   Definition modsems: list ModSem := [program_to_ModSem program]. 
-  
-  (*
-    Definition isem: itree Event unit :=
-      eval_multimodule_multicore
-        modsems [ "main" ; "alloc1F" ; "alloc2F" ].
-   *)
-  
+   
 End HighSpecDummyTest.
 
+Module AbsData.
+
+  (* MPOOL_DEFINITION *)
+
+  Definition ident := N.
+
+  Instance RelDec_ident: RelDec (@eq ident) :=
+    { rel_dec := fun n0 n1 => if (N.eqb n0 n1) then true else false}.
+
+  (* mpool *)
+
+  Record mpool: Type :=
+    mkMPOOL {
+        chunk_addr: option N;
+        chunk_limit: N;
+        fallback: option ident; (* mpoolid *)
+      }
+  .
+  
+
+  Definition GMPOOL := (Map mpool).
+    
+  Definition mp_manager: Type := ident -> option GMPOOL.
+  Definition inital_mp_manager: mp_manager := fun _ => None.
+  Definition mp_update (m: mp_manager) (k0: ident) (v: option GMPOOL): mp_manager :=
+    fun k1 => if rel_dec k0 k1 then v else m k1
+  .
 
 
-(*
-Module MPOOLMMHIGHTest.
 
-  Let mpool_init_aux (vs: list val): (val * list val) :=
+  (* PTE Definition *)
+  (* 
+  /* The following are arch-independent page mapping modes. */
+  #define MM_MODE_R UINT32_C(0x0001) /* read */
+  #define MM_MODE_W UINT32_C(0x0002) /* write */
+  #defi   ne MM_MODE_X UINT32_C(0x0004) /* execute */
+  #define    MM_MODE_D UINT32_C(0x0008) /* device */
+   *)
+  
+  (* The following are arch-independent page mapping modes. *)
+  Inductive ModeFlag :=
+  | MM_MODE_UNDEF (* nothing *)
+  | MM_MODE_R (* read *)
+  | MM_MODE_W (* write *)
+  | MM_MODE_X (* execute *)
+  | MM_MODE_D (* device *)
+  .
+  
+  (*
+/*
+ * Memory in stage-1 is either valid (present) or invalid (absent).
+ *
+ * Memory in stage-2 has more states to track sharing, borrowing and giving of
+ * memory. The states are made up of three parts:
+ *
+ *  1. V = valid/invalid    : Whether the memory is part of the VM's address
+ *                            space. A fault will be generated if accessed when
+ *                            invalid.
+ *  2. O = owned/unowned    : Whether the memory is owned by the VM.
+ *  3. X = exclusive/shared : Whether access is exclusive to the VM or shared
+ *                            with at most one other.
+ *
+ * These parts compose to form the following state:
+ *
+ *  -  V  O  X : Owner of memory with exclusive access.
+ *  -  V  O !X : Owner of memory with access shared with at most one other VM.
+ *  -  V !O  X : Borrower of memory with exclusive access.
+ *  -  V !O !X : Borrower of memory where access is shared with the owner.
+ *  - !V  O  X : Owner of memory lent to a VM that has exclusive access.
+ *
+ *  - !V  O !X : Unused. Owner of shared memory always has access.
+ *  - !V !O  X : Unused. Next entry is used for invalid memory.
+ *
+ *  - !V !O !X : Invalid memory. Memory is unrelated to the VM.
+ *
+ *  Modes are selected so that owner of exclusive memory is the default.
+ */
+#define MM_MODE_INVALID UINT32_C(0x0010)
+#define MM_MODE_UNOWNED UINT32_C(0x0020)
+#define MM_MODE_SHARED  UINT32_C(0x0040)
+   *)
+  
+  Inductive OwnModeFlag :=
+  | MM_OWN_MODE_UNDEF
+  | MM_MODE_INVALID
+  | MM_MODE_UNOWNED
+  | MM_MODE_SHARED.
+
+  Definition ADDR_VAL :=  N. (* we may need an invariant to figure out the range of the address *)
+
+  Inductive PTE_TY :=
+  | PTE_UNDEF
+  | PTE_ABSENT (addr: N)
+  | PTE_VALID (addr: N) (block_addr: N) (mf: ModeFlag) (omf: OwnModeFlag).
+  (* addr is the base address of the PTE *)
+  
+  Definition PT := (Map PTE_TY).
+  
+  Record ST1PTP :=
+    mkST1PTP {
+        st1_root_table: PTE_TY;
+        st1l1pt : PT;
+        st1l0pt : PT
+      }.
+  
+  Record ST2PTP :=
+    mkST2PTP {
+        st2_root_table: PTE_TY;
+        st2l2pt : PT;
+        st2l1pt : PT;
+        st2l0pt : PT
+      }.
+
+  Inductive PTP_TY :=
+  | PTP_ST1 (ptp_st1: ST1PTP)
+  | PTP_ST2 (ptp_st2: ST2PTP).
+
+ 
+  Definition GPTP := (Map PTP_TY).
+
+  Definition pt_manager : Type := ident -> option GPTP.
+  Definition inital_pt_manager: mp_manager := fun _ => None.
+  Definition pt_update (m: pt_manager) (k0: ident) (v: option GPTP): pt_manager :=
+    fun k1 => if rel_dec k0 k1 then v else m k1
+  .
+
+End AbsData.
+
+Module PTHIGH.
+
+  Include AbsData.
+
+  Definition TEST_HEAP_SIZE := 1024%N. 
+  Definition pte_paddr_begin := 4000%N.
+  Definition entry_size := 16.
+  Definition root_id := 0.
+  Definition thread_set := [1; 2].
+  
+  Definition init_mpool (base_addr: option N) (curid : ident) (pid: ident) (limit: N) : mpool :=
+    {| chunk_addr := base_addr;
+       chunk_limit := (entry_size * limit)%N;
+       fallback := if (eq_dec root_id curid) then None else Some pid |}.
+
+  Definition init_ST1PTP (addr: N) :=
+    {| st1_root_table := PTE_ABSENT addr;
+       st1l1pt := (newMap PTE_TY);
+       st1l0pt := (newMap PTE_TY) |}.                    
+
+  Definition init_ST2PTP (addr: N) :=
+    {| st2_root_table := PTE_ABSENT addr;
+       st2l2pt := (newMap PTE_TY);
+       st2l1pt := (newMap PTE_TY);
+       st2l0pt := (newMap PTE_TY) |}.                    
+  
+  Definition init_ptp (nid: ident) (stage: N) (addr: N) :=
+    if (eq_dec stage 1)
+    then (PTP_ST1 (init_ST1PTP addr))
+    else (PTP_ST2 (init_ST2PTP addr)).
+
+  Definition root_map := (MapPut mpool) (newMap mpool) root_id (init_mpool (Some  pte_paddr_begin) root_id root_id TEST_HEAP_SIZE).
+
+  Fixpoint initialize_mpool (l: list N) (init_map : (Map mpool)) :=
+    match l with
+    | nil => init_map
+    | hd::tl => let res := initialize_mpool tl init_map in
+                (MapPut mpool) res hd (init_mpool None hd root_id 0)
+    end.
+                
+  Definition init_mp := initialize_mpool thread_set root_map.
+
+  Let mpool_init  (vs : list val@{expr.u1}): (val@{expr.u2} * list val@{expr.u3}) :=
     let retv := match vs with
-                | [(Vabs a) ; (Vptr (Some p_id) _)] =>
-                  match downcast a mp_manager with
-                  | Some mm0 => let mm1 := (mp_update mm0 p_id (Some (mk nil None))) in
-                                Vabs (upcast mm1)
-                  | _ => Vnodef
-                  end
+                | nil =>
+                  unwrap (let new_mp := init_mp in
+                          Some (Vabs (upcast new_mp))) Vnodef
                 | _ => Vnodef
                 end
     in
-    (retv, nil)
-  .
-  
-  Definition mpool_init (p: var) r: stmt :=
-    r #= GetOwnedHeap #;
-      PutOwnedHeap (CoqCode [CBV r ; CBV p] mpool_init_aux) #;
-      Skip
-  .
+    (retv, nil).
 
-
-
-  Let mp_init_with_fallback_aux (vs: list val): (val * list val) :=
+  Let ptp_init  (vs : list val@{expr.u1}): (val@{expr.u2} * list val@{expr.u3}) :=
     let retv := match vs with
-                | [(Vabs a) ; (Vptr (Some p_id) _) ; (Vptr (Some fb_id) _)] =>
-                  match downcast a mp_manager with
-                  | Some mm0 => let mm1 := (mp_update mm0 p_id (Some (mk nil (Some fb_id)))) in
-                                Vabs (upcast mm1)
-                  | _ => Vnodef
-                  end
+                | nil =>
+                  unwrap (let new_mp := init_mp in
+                          Some (Vabs (upcast (newMap PTP_TY)))) Vnodef
                 | _ => Vnodef
                 end
     in
-    (retv, nil)
-  .
+    (retv, nil).
   
-  Definition mpool_init_with_fallback (p fallback: var) r: stmt :=
-    r #= GetOwnedHeap #;
-      PutOwnedHeap (CoqCode [CBV r ; CBV p ; CBV fallback] mp_init_with_fallback_aux) #;
-      Skip
-  .
+End PTHIGH.
+
+Module PTHIGHTEST.
+
+  Include PTHIGH.
+   
+  Definition main mp ptp : stmt :=
+    Eval compute in INSERT_YIELD (    
+      (DebugHigh "[high-model] Calling ptable_init" Vnull) #;
+      mp #= (CoqCode [] mpool_init) #;
+      ptp #= (CoqCode [] ptp_init) #;
+      (DebugHigh "[high-model] End ptable_init" Vnull)).
+
+
+  Definition ptable_init : stmt :=
+    Eval compute in INSERT_YIELD (Skip).    
+
+
+  Definition mainF: function.
+    mk_function_tac main ([]: list var) (["mp" ; "ptp"] : list var).
+  Defined.
+
+  Definition ptable_initF: function.
+    mk_function_tac ptable_init ([]: list var) ([] : list var).
+  Defined.
+
   
-  Let mpool_check_fallback (vs: list val): (val * list val) :=
-    let retv := match vs with
-                | [(Vabs a) ; (Vptr (Some p_id) _)]=>
-                  unwrap (mm <- downcast a mp_manager ;;
-                          mp <- mm p_id ;;
-                          Some (is_some (mp.(fallback)): val)
-                         ) Vnodef
-                | _ => Vnodef
-                end
-    in
-    (retv, nil)
-  .
+  Definition program: program :=
+    [
+      ("main", mainF) ;
+    ("ptable_init", ptable_initF)
+    ].
   
-  Let mpool_get_chunk_list (vs: list val): (val * list val) :=
-    let retv := match vs with
-                | [(Vabs a) ; (Vptr (Some p_id) _)]=>
-                  unwrap (mm <- downcast a mp_manager ;;
-                          mp <- mm p_id ;;
-                          Some (Vabs (upcast mp.(chunklist)))
-                         ) Vnodef
-                | _ => Vnodef
-                end
-    in
-    (retv, nil)
-  .
-  
-  Definition mpool_add_chunk (mp: mpool) (chunk: nat * nat): mpool :=
-    mk (chunk :: mp.(chunklist)) mp.(fallback)
+  Definition isem: itree Event unit :=
+    eval_multimodule [program_to_ModSem program]
+      (* eval_multimodule [LOCK.modsem ; program_to_ModSem program] *)
   .
 
-  Let mp_fini_aux (vs: list val): (val * list val) :=
-    match vs with
-    | [(Vabs a0) ; (Vptr (Some p_id) _) ; (Vabs a1)]=>
-      unwrap (mm0 <- downcast a0 mp_manager ;;
-              cl <- downcast a1 (list (nat * nat)) ;;
-              mp <- mm0 p_id ;;
-              fb_id <- mp.(fallback) ;;
-              fb <- mm0 fb_id ;;
-              match cl with
-              | hd :: tl =>
-                let mm1 := (mp_update mm0 fb_id (Some (mpool_add_chunk fb hd))) in
-                Some (Vtrue, [(Vabs (upcast mm1)) ; (Vabs (upcast tl))])
-              | _ => Some (Vfalse, [(Vabs a0) ; (Vabs a1)])
-              (* | _ => (Vfalse, [(Vabs (upcast mm0)) ; (Vabs (upcast nil))]) *)
-              end
-             ) (Vnodef, nil)
-    | _ => (Vnodef, nil)
-    end
-  .
+End PTHIGHTEST.
 
-  Let fini_aux2 (vs: list val): (val * list val) :=
-    let retv := match vs with
-                | [(Vabs a) ; (Vptr (Some p_id) _)]=>
-                  unwrap (mm0 <- downcast a mp_manager ;;
-                          mp <- mm0 p_id ;;
-                          let mm1 := (mp_update mm0 p_id None) in
-                          Some (Vabs (upcast mm1))
-                         ) Vnodef
-                | _ => Vnodef
-                end
-    in
-    (retv, nil)
-  .
 
-End MPOOLMMHIGHTest.
-*)
+Section ADDR_TRANSLATION.
+    
+  (* This one is for later implementation *)
+  
+  (*  This is the wrapper definition for va_addr to distinguish it with normal natural numbers -
+     We can remove some of them later *)
+  Inductive va_addr :=
+  | VA_ADDR (va: N).
+
+  Inductive ipa_addr :=
+  | IPA_ADDR (ipa: N).
+
+  (* Low level functional model for mm_index *)
+  (*
+  Definition mm_index (addr level: var) (v  : var) : stmt :=
+    v #= addr #>> (PAGE_BITS + (level * PAGE_LEVEL_BITS)) #;
+      Return (v #& ((UINT64_C(1) #<< PAGE_LEVEL_BITS) - 1)).
+   *)
+
+  (* high-level functional model for mm_index - It is quite same. we just change the definition as a normal Coq definition  *)
+  Definition h_mm_index  (va : va_addr) (level : N) : N :=
+    match va with
+    | VA_ADDR va' =>
+      let v := (N.shiftr va' ((level * PAGE_LEVEL_BITS)%N + PAGE_BITS)%N) in
+      let mask := (N.shiftl 1 PAGE_LEVEL_BITS) - 1 in
+      (N.land v mask) 
+    end.
+
+  Definition va_page_bits (va: va_addr) : N :=
+    match va with
+    | VA_ADDR va' =>
+      let mask := (N.shiftl 1 PAGE_BITS) - 1 in
+      (N.land va' mask)
+    end.
+
+  Definition ipa_block_idx (level : N) (ipa : ipa_addr) : N :=
+    match ipa with
+    | IPA_ADDR ipa' =>
+      let mask := (N.shiftl 1 PAGE_LEVEL_BITS) - 1 in
+      (N.land (N.shiftr ipa' ((level * PAGE_LEVEL_BITS)%N + PAGE_BITS)%N) mask) 
+    end.
+ 
+End ADDR_TRANSLATION.
+
